\documentclass{article}
\usepackage{amsmath,amsfonts}
\begin{document}
\noindent $e$ is distributed according to the PDF
\begin{equation}
	f(e)=x(e)^{a-1}(1-x(e))^{b-1}
\end{equation}
where
\begin{equation}
	x(e)=\frac{1}{2}\left[1+\frac{e}{\bar{e}}\right]
\end{equation}
We want
\begin{align}
	I_{k}(\widetilde{m})&=\int_{\alpha}^{\beta}{q^{k}f(\tilde{m}-q)dq}\\
	&=\int_{\alpha}^{\beta}{q^{k}x(\tilde{m}-q)^{a-1}(1-x(\tilde{m}-q))^{b-1}dq}\\
\end{align}
Note that the normalizing constant cancels out when computing the conditional expectation. 
\end{document}
