\documentclass[12pt]{article}
\usepackage{amsmath,amssymb,amsfonts,fullpage,setspace}
\begin{document}
\onehalfspacing
\noindent The noise, $\epsilon$, has support $[-\bar{\epsilon},\bar{\epsilon}]$ and is distributed according to the PDF
\begin{equation}
g(e;\alpha,\beta)=g(\alpha,\beta)^{-1}(e+\bar{\epsilon})^{\alpha-1}(e-\bar{\epsilon})^{\beta-1}
\end{equation}
where
\begin{equation}
G(\alpha,\beta)=\int_{-\bar{\epsilon}}^{\bar{\epsilon}}{(\bar{\epsilon}+e)^{\alpha-1}(\bar{\epsilon}-e)^{\beta-1}de}.
\end{equation}
$g$ is just the PDF of the Beta distribution with support $[-\bar{\epsilon},\bar{\epsilon}]$. Put $x=(\bar{\epsilon}+e)/2\bar{\epsilon}$ and observe that
\begin{align}
G(\alpha,\beta)&=\int_{0}^{1}{(2\bar{\epsilon}x)^{\alpha-1}(\bar{\epsilon}-(2\bar{\epsilon}x-\bar{\epsilon}))^{\beta-1}2\bar{\epsilon}dx}\\
&=(2\bar{\epsilon})^{\alpha+\beta-1}\int_{0}^{1}{x^{\alpha-1}(1-x)^{\beta-1}dx}\\
&=(2\bar{\epsilon})^{\alpha+\beta-1}B(\alpha,\beta)
\end{align}
where $B$ is the beta function. We require that $\epsilon$ has mean zero:
\begin{equation}
0=E[\epsilon]=\int_{-\bar{\epsilon}}^{\bar{\epsilon}}{e(e+\bar{\epsilon})^{\alpha}(e-\bar{\epsilon})^{\beta}de}=\frac{\alpha}{\alpha+\beta}. 
\end{equation}
Hence, $\epsilon$ has variance 
\begin{equation}
0=E[\epsilon^{2}]=\int_{-\bar{\epsilon}}^{\bar{\epsilon}}{e^{2}(e+\bar{\epsilon})^{\alpha}(e-\bar{\epsilon})^{\beta}de}
\end{equation}
\end{document}