\documentclass{article}
\usepackage{amsmath,amsfonts}
\begin{document}
\noindent Let $x:[-\overline{e},\overline{e}]\rightarrow[0,1]$ be given by
\begin{equation}
	x(e)=\frac{1}{2}\left[1+\frac{e}{\overline{e}}\right]
\end{equation}
Define
\begin{align}
	I_{(\alpha,\beta,\gamma)}(\widetilde{m})\equiv\int_{\alpha}^{\beta}{q^{\gamma}f(\tilde{m}-q)dq}
\end{align}
and
\begin{equation}
	A(\widetilde{m})=
	\begin{cases}
		\overline{a}(\widetilde{m}) & \text{ if } 1-\overline{e}<\widetilde{m}\leq 1+\overline{e}\\
		a(\widetilde{m}) & \text{ if } \overline{e}<\widetilde{m}\leq 1-\overline{e}\\
		\underline{a}(\widetilde{m}) & \text{ if } -\overline{e}\leq\widetilde{m}\leq \overline{e}
	\end{cases}
\end{equation}
where
\begin{align}
	\overline{a}(\widetilde{m})&=\frac{I_{(\widetilde{m}-\bar{e},1,1)}(\widetilde{m})}{I_{(\widetilde{m}-\bar{e},1,0)}(\widetilde{m})}\\
	a(\widetilde{m})&=\frac{I_{(\widetilde{m}-\bar{e},\widetilde{m}+\bar{e},1)}(\widetilde{m})}{I_{(\widetilde{m}-\bar{e},\widetilde{m}+\bar{e},0)}(\widetilde{m})}\\
	\underline{a}(\widetilde{m})&=\frac{I_{(0,\widetilde{m}+\bar{e},1)}(\widetilde{m})}{I_{(0,\widetilde{m}+\bar{e},0)}(\widetilde{m})}
\end{align}
Note that the normalizing constant cancels out when computing the conditional expectation. We need three sets of weights and knots. The cost is given by
\begin{align}
	C[m_{i}]&=\int_{-\bar{e}}^{1+\bar{e}}{\int_{q_{-}(\widetilde{m})}^{q_{+}(\widetilde{m})}{(q-A(\widetilde{m}))^{2}f(\widetilde{m}-q)dq}d\widetilde{m}}.
\end{align}
where
\begin{align}
	q_{+}(\widetilde{m})&=\min\{\widetilde{m}+\bar{e},1\}\\
	q_{-}(\widetilde{m})&=\max\{\widetilde{m}-\bar{e},0\}
\end{align}
Define
\begin{align}
	\overline{z}&=\int_{1-\bar{e}}^{1+\bar{e}}{\int_{\widetilde{m}-\bar{e}}^{1}{(q-\overline{a}(\widetilde{m}))^{2}f(\widetilde{m}-q)dq}d\widetilde{m}}\\
	z&=\int_{\bar{e}}^{1-\bar{e}}{\int_{\widetilde{m}-\bar{e}}^{\widetilde{m}+\bar{e}}{(q-a(\widetilde{m}))^{2}f(\widetilde{m}-q)dq}d\widetilde{m}}\\
	\underline{z}&=\int_{-\bar{e}}^{\bar{e}}{\int_{0}^{\widetilde{m}+\bar{e}}{(q-\underline{a}(\widetilde{m}))^{2}f(\widetilde{m}-q)dq}d\widetilde{m}}
\end{align}
Consider, as an example, the Beta PDF:
\begin{equation}
	f(e)=x(e)^{a-1}(1-x(e))^{b-1}
\end{equation}
for constants $a>0$ and $b>0$. 
\end{document}
